coq_inference/hoare.v
@@ -53,13 +53,13 @@ Module Hoare(L : LanguageDef).
       is_call (χ, ψ) x (m_call α m ((local ϕ) ∘ β)).
 
   Inductive hoare_triple : mdl -> asrt -> meth_call -> asrt -> Prop :=
-  | ht_r : forall M1 α m β P Q, (forall M2 x σ σ', is_call σ x (m_call α m β) ->
-                                       M1 ⦂ M2 ◎ σ ⊨ P ->
-                                       M1 ⦂ M2 ⦿ σ ⤳ σ' ->
-                                       exists v χ ϕ ψ, σ' = (χ, ϕ :: ψ) /\
+  | ht_r : forall M α m β P Q, (forall M' x σ σ', is_call σ x (m_call α m β) ->
+                                        M ◎ σ ⊨ P ->
+                                        M ⦂ M' ⦿ σ ⤳ σ' ->
+                                        exists v χ ϕ ψ, σ' = (χ, ϕ :: ψ) /\
                                                   ⟦ x ↦ v ⟧_∈ local ϕ /\
-                                                  M1 ⦂ M2 ◎ σ' ⊨ [v /s 0]Q) ->
-                       M1 ⊢ {pre: P} (m_call α m β) {post: Q}
+                                                  M ◎ σ' ⊨ [v /s 0]Q) ->
+                          M ⊢ {pre: P} (m_call α m β) {post: Q}
 
   where "M '⊢' '{pre:' P '}' m '{post:' Q '}'"
           := (hoare_triple M P m Q).
